Finish completeness (#90)
* Use better tactic

* Finish natrec cong case

* Add all completeness lemma statements

* Prove nat_beta_zero

* Finish nat cases for completeness

* Do minor renaming

* Add hints

* Add mutual induction principle for syntactic system

* Prove completeness fundamental theorem

* Prove the main theorem

* Add the missing file

* Update proofs

* Rename inconsistent relation

* Fix some proofs

* Fix a_sub

* Remove an unnecessary lemma

theories/Core/Completeness/LogicalRelation/Definitions.v
@@ -7,6 +7,8 @@ Inductive rel_exp M p M' p' (R : relation domain) : Prop :=
 | mk_rel_exp : forall m m', {{ ⟦ M ⟧ p ↘ m }} -> {{ ⟦ M' ⟧ p' ↘ m' }} -> {{ Dom m ≈ m' ∈ R }} -> rel_exp M p M' p' R.
 #[global]
 Arguments mk_rel_exp {_ _ _ _ _}.
+#[export]
+Hint Constructors rel_exp : mcltt.
 
 Definition rel_exp_under_ctx Γ A M M' :=
   exists env_rel (_ : {{ EF Γ ≈ Γ ∈ per_ctx_env ↘ env_rel }}) i,
@@ -17,25 +19,35 @@ Definition rel_exp_under_ctx Γ A M M' :=
 Definition valid_exp_under_ctx Γ A M := rel_exp_under_ctx Γ A M M.
 #[global]
 Arguments valid_exp_under_ctx _ _ _ /.
+#[export]
+Hint Transparent valid_exp_under_ctx : mcltt.
+#[export]
+Hint Unfold valid_exp_under_ctx : mcltt.
 
-Inductive rel_subst σ p σ' p' (R : relation env) : Prop :=
-| mk_rel_subst : forall o o', {{ ⟦ σ ⟧s p ↘ o }} -> {{ ⟦ σ' ⟧s p' ↘ o' }} -> {{ Dom o ≈ o' ∈ R }} -> rel_subst σ p σ' p' R.
+Inductive rel_sub σ p σ' p' (R : relation env) : Prop :=
+| mk_rel_sub : forall o o', {{ ⟦ σ ⟧s p ↘ o }} -> {{ ⟦ σ' ⟧s p' ↘ o' }} -> {{ Dom o ≈ o' ∈ R }} -> rel_sub σ p σ' p' R.
 #[global]
-Arguments mk_rel_subst {_ _ _ _ _ _}.
+Arguments mk_rel_sub {_ _ _ _ _ _}.
+#[export]
+Hint Constructors rel_sub : mcltt.
 
-Definition rel_subst_under_ctx Γ Δ σ σ' :=
+Definition rel_sub_under_ctx Γ Δ σ σ' :=
   exists env_rel (_ : {{ EF Γ ≈ Γ ∈ per_ctx_env ↘ env_rel }})
      env_rel' (_ : {{ EF Δ ≈ Δ ∈ per_ctx_env ↘ env_rel' }}),
   forall p p' (equiv_p_p' : {{ Dom p ≈ p' ∈ env_rel }}),
-    rel_subst σ p σ' p' env_rel'.
+    rel_sub σ p σ' p' env_rel'.
 
-Definition valid_subst_under_ctx Γ Δ σ := rel_subst_under_ctx Γ Δ σ σ.
+Definition valid_sub_under_ctx Γ Δ σ := rel_sub_under_ctx Γ Δ σ σ.
 #[global]
-Arguments valid_subst_under_ctx _ _ _ /.
+Arguments valid_sub_under_ctx _ _ _ /.
+#[export]
+Hint Transparent valid_sub_under_ctx : mcltt.
+#[export]
+Hint Unfold valid_sub_under_ctx : mcltt.
 
 Notation "⊨ Γ ≈ Γ'" := (per_ctx Γ Γ')  (in custom judg at level 80, Γ custom exp, Γ' custom exp).
 Notation "⊨ Γ" := (valid_ctx Γ) (in custom judg at level 80, Γ custom exp).
 Notation "Γ ⊨ M ≈ M' : A" := (rel_exp_under_ctx Γ A M M') (in custom judg at level 80, Γ custom exp, M custom exp, M' custom exp, A custom exp).
 Notation "Γ ⊨ M : A" := (valid_exp_under_ctx Γ A M) (in custom judg at level 80, Γ custom exp, M custom exp, A custom exp).
-Notation "Γ ⊨s σ ≈ σ' : Δ" := (rel_subst_under_ctx Γ Δ σ σ') (in custom judg at level 80, Γ custom exp, σ custom exp, σ' custom exp, Δ custom exp).
-Notation "Γ ⊨s σ : Δ" := (valid_subst_under_ctx Γ Δ σ) (in custom judg at level 80, Γ custom exp, σ custom exp, Δ custom exp).
+Notation "Γ ⊨s σ ≈ σ' : Δ" := (rel_sub_under_ctx Γ Δ σ σ') (in custom judg at level 80, Γ custom exp, σ custom exp, σ' custom exp, Δ custom exp).
+Notation "Γ ⊨s σ : Δ" := (valid_sub_under_ctx Γ Δ σ) (in custom judg at level 80, Γ custom exp, σ custom exp, Δ custom exp).
