theories/Core/Completeness.v
@@ -1,0 +1,20 @@
+From Mcltt Require Import Base LibTactics.
+From Mcltt.Core Require Import Completeness.LogicalRelation Completeness.FundamentalTheorem Semantic.NbE Semantic.Realizability System.
+Import Domain_Notations.
+
+Theorem completeness : forall {Γ M M' A},
+  {{ Γ ⊢ M ≈ M' : A }} ->
+  exists m, nbe Γ M A m /\ nbe Γ M' A m.
+Proof with mautosolve.
+  intros * [env_relΓ]%completeness_fundamental_exp_eq.
+  destruct_conjs.
+  assert (exists p p', initial_env Γ p /\ initial_env Γ p' /\ {{ Dom p ≈ p' ∈ env_relΓ }}) as [p] by (apply per_ctx_then_per_env_initial_env; eauto).
+  destruct_conjs.
+  functional_initial_env_rewrite_clear.
+  (on_all_hyp: destruct_rel_by_assumption env_relΓ).
+  rename x into elem_rel.
+  destruct_by_head rel_typ.
+  functional_eval_rewrite_clear.
+  destruct_by_head rel_exp.
+  unshelve epose proof (per_elem_then_per_top _ _ (length Γ)) as [? []]; shelve_unifiable...
+Qed.
