theories/Core/Completeness/SubstitutionCases.v
@@ -3,49 +3,56 @@ From Mcltt Require Import Base LibTactics.
 From Mcltt.Core Require Import Completeness.ContextCases Completeness.LogicalRelation System.
 Import Domain_Notations.
 
-Lemma rel_subst_id : forall {Γ},
+Lemma rel_sub_id : forall {Γ},
     {{ ⊨ Γ }} ->
     {{ Γ ⊨s Id ≈ Id : Γ }}.
-Proof with intuition.
+Proof with mautosolve.
   intros * [].
-  eexists_rel_subst.
-  econstructor; only 1-2: repeat econstructor...
+  eexists_rel_sub...
 Qed.
 
-Lemma rel_subst_weaken : forall {Γ A},
+#[export]
+Hint Resolve rel_sub_id : mcltt.
+
+Lemma rel_sub_weaken : forall {Γ A},
     {{ ⊨ Γ, A }} ->
     {{ Γ, A ⊨s Wk ≈ Wk : Γ }}.
 Proof with intuition.
   intros * [env_relΓA].
   inversion_by_head (per_ctx_env env_relΓA); subst.
-  eexists_rel_subst.
+  eexists_rel_sub.
   econstructor; only 1-2: repeat econstructor...
 Qed.
 
-Lemma rel_subst_compose_cong : forall {Γ τ τ' Γ' σ σ' Γ''},
+#[export]
+Hint Resolve rel_sub_weaken : mcltt.
+
+Lemma rel_sub_compose_cong : forall {Γ τ τ' Γ' σ σ' Γ''},
     {{ Γ ⊨s τ ≈ τ' : Γ' }} ->
     {{ Γ' ⊨s σ ≈ σ' : Γ'' }} ->
     {{ Γ ⊨s σ ∘ τ ≈ σ' ∘ τ' : Γ'' }}.
-Proof with intuition.
+Proof with mautosolve.
   pose proof (@relation_equivalence_pointwise domain).
   pose proof (@relation_equivalence_pointwise env).
   intros * [env_relΓ [? [env_relΓ']]] [].
   destruct_conjs.
   pose (env_relΓ'0 := env_relΓ').
   handle_per_ctx_env_irrel.
-  eexists_rel_subst.
+  eexists_rel_sub.
   intros.
   (on_all_hyp: destruct_rel_by_assumption env_relΓ).
-  (on_all_hyp: destruct_rel_by_assumption env_relΓ').
-  econstructor; only 1-2: repeat econstructor...
+  (on_all_hyp: destruct_rel_by_assumption env_relΓ')...
 Qed.
 
-Lemma rel_subst_extend_cong : forall {i Γ M M' σ σ' Δ A},
+#[export]
+Hint Resolve rel_sub_compose_cong : mcltt.
+
+Lemma rel_sub_extend_cong : forall {i Γ M M' σ σ' Δ A},
     {{ Γ ⊨s σ ≈ σ' : Δ }} ->
     {{ Δ ⊨ A : Type@i }} ->
     {{ Γ ⊨ M ≈ M' : A[σ] }} ->
     {{ Γ ⊨s σ ,, M ≈ σ' ,, M' : Δ, A }}.
-Proof with intuition.
+Proof with mautosolve.
   pose proof (@relation_equivalence_pointwise domain).
   pose proof (@relation_equivalence_pointwise env).
   intros * [env_relΓ [? [env_relΔ]]] HA [].
@@ -56,7 +63,7 @@ Proof with intuition.
   destruct_conjs.
   pose (env_relΔA0 := env_relΔA).
   handle_per_ctx_env_irrel.
-  eexists_rel_subst.
+  eexists_rel_sub.
   match_by_head (per_ctx_env env_relΔA) invert_per_ctx_env.
   destruct_conjs.
   handle_per_ctx_env_irrel.
@@ -66,40 +73,46 @@ Proof with intuition.
   destruct_by_head rel_typ.
   inversion_by_head (eval_exp {{{ A[σ] }}}); subst.
   handle_per_univ_elem_irrel.
-  destruct_by_head rel_exp.
-  econstructor; only 1-2: repeat econstructor; eauto.
+  destruct_by_head rel_exp...
 Qed.
 
-Lemma rel_subst_id_compose_right : forall {Γ σ Δ},
+#[export]
+Hint Resolve rel_sub_extend_cong : mcltt.
+
+Lemma rel_sub_id_compose_right : forall {Γ σ Δ},
     {{ Γ ⊨s σ : Δ }} ->
     {{ Γ ⊨s Id ∘ σ ≈ σ : Δ }}.
-Proof with intuition.
+Proof with mautosolve.
   intros * [env_relΓ].
   destruct_conjs.
-  eexists_rel_subst.
+  eexists_rel_sub.
   intros.
-  (on_all_hyp: destruct_rel_by_assumption env_relΓ).
-  econstructor; only 1-2: repeat econstructor...
+  (on_all_hyp: destruct_rel_by_assumption env_relΓ)...
 Qed.
 
-Lemma rel_subst_id_compose_left : forall {Γ σ Δ},
+#[export]
+Hint Resolve rel_sub_id_compose_right : mcltt.
+
+Lemma rel_sub_id_compose_left : forall {Γ σ Δ},
     {{ Γ ⊨s σ : Δ }} ->
     {{ Γ ⊨s σ ∘ Id ≈ σ : Δ }}.
-Proof with intuition.
+Proof with mautosolve.
   intros * [env_relΓ].
   destruct_conjs.
-  eexists_rel_subst.
+  eexists_rel_sub.
   intros.
-  (on_all_hyp: destruct_rel_by_assumption env_relΓ).
-  econstructor; only 1-2: repeat econstructor...
+  (on_all_hyp: destruct_rel_by_assumption env_relΓ)...
 Qed.
 
-Lemma rel_subst_compose_assoc : forall {Γ σ Γ' σ' Γ'' σ'' Γ'''},
+#[export]
+Hint Resolve rel_sub_id_compose_left : mcltt.
+
+Lemma rel_sub_compose_assoc : forall {Γ σ Γ' σ' Γ'' σ'' Γ'''},
     {{ Γ' ⊨s σ : Γ }} ->
     {{ Γ'' ⊨s σ' : Γ' }} ->
     {{ Γ''' ⊨s σ'' : Γ'' }} ->
     {{ Γ''' ⊨s (σ ∘ σ') ∘ σ'' ≈ σ ∘ (σ' ∘ σ'') : Γ }}.
-Proof with intuition.
+Proof with mautosolve.
   pose proof (@relation_equivalence_pointwise domain).
   pose proof (@relation_equivalence_pointwise env).
   intros * [env_relΓ' [? [env_relΓ]]] [env_relΓ'' [? []]] [env_relΓ'''].
@@ -107,21 +120,24 @@ Proof with intuition.
   pose (env_relΓ'0 := env_relΓ').
   pose (env_relΓ''0 := env_relΓ'').
   handle_per_ctx_env_irrel.
-  eexists_rel_subst.
+  eexists_rel_sub.
   intros.
   (on_all_hyp: destruct_rel_by_assumption env_relΓ''').
   (on_all_hyp: destruct_rel_by_assumption env_relΓ'').
   (on_all_hyp: destruct_rel_by_assumption env_relΓ').
-  econstructor; only 1-2: repeat econstructor...
+  econstructor...
 Qed.
 
-Lemma rel_subst_extend_compose : forall {Γ τ Γ' M σ Γ'' A i},
+#[export]
+Hint Resolve rel_sub_compose_assoc : mcltt.
+
+Lemma rel_sub_extend_compose : forall {Γ τ Γ' M σ Γ'' A i},
     {{ Γ' ⊨s σ : Γ'' }} ->
     {{ Γ'' ⊨ A : Type@i }} ->
     {{ Γ' ⊨ M : A[σ] }} ->
     {{ Γ ⊨s τ : Γ' }} ->
     {{ Γ ⊨s (σ ,, M) ∘ τ ≈ (σ ∘ τ) ,, M[τ] : Γ'', A }}.
-Proof with intuition.
+Proof with mautosolve.
   pose proof (@relation_equivalence_pointwise domain).
   pose proof (@relation_equivalence_pointwise env).
   intros * [env_relΓ' [? [env_relΓ'']]] HA [] [env_relΓ].
@@ -132,7 +148,7 @@ Proof with intuition.
   destruct_conjs.
   pose (env_relΓ''A0 := env_relΓ''A).
   handle_per_ctx_env_irrel.
-  eexists_rel_subst.
+  eexists_rel_sub.
   match_by_head (per_ctx_env env_relΓ''A) invert_per_ctx_env.
   destruct_conjs.
   handle_per_ctx_env_irrel.
@@ -144,14 +160,17 @@ Proof with intuition.
   inversion_by_head (eval_exp {{{ A[σ] }}}); subst.
   handle_per_univ_elem_irrel.
   destruct_by_head rel_exp.
-  econstructor; only 1-2: repeat econstructor; try eexists...
+  econstructor...
 Qed.
 
-Lemma rel_subst_p_extend : forall {Γ' M σ Γ A},
+#[export]
+Hint Resolve rel_sub_extend_compose : mcltt.
+
+Lemma rel_sub_p_extend : forall {Γ' M σ Γ A},
     {{ Γ' ⊨s σ : Γ }} ->
     {{ Γ' ⊨ M : A[σ] }} ->
     {{ Γ' ⊨s Wk ∘ (σ ,, M) ≈ σ : Γ }}.
-Proof with intuition.
+Proof with mautosolve.
   pose proof (@relation_equivalence_pointwise domain).
   pose proof (@relation_equivalence_pointwise env).
   intros * [env_relΓ' [? [env_relΓ]]] [].
@@ -159,20 +178,23 @@ Proof with intuition.
   pose (env_relΓ0 := env_relΓ).
   pose (env_relΓ'0 := env_relΓ').
   handle_per_ctx_env_irrel.
-  eexists_rel_subst.
+  eexists_rel_sub.
   intros.
   (on_all_hyp: destruct_rel_by_assumption env_relΓ').
   destruct_by_head rel_typ.
   inversion_by_head (eval_exp {{{ A[σ] }}}); subst.
   handle_per_univ_elem_irrel.
   destruct_by_head rel_exp.
-  econstructor; only 1-2: repeat econstructor...
+  econstructor...
 Qed.
 
-Lemma rel_subst_extend : forall {Γ' σ Γ A},
+#[export]
+Hint Resolve rel_sub_p_extend : mcltt.
+
+Lemma rel_sub_extend : forall {Γ' σ Γ A},
     {{ Γ' ⊨s σ : Γ, A }} ->
     {{ Γ' ⊨s σ ≈ (Wk ∘ σ) ,, #0[σ] : Γ, A }}.
-Proof with intuition.
+Proof with mautosolve.
   pose proof (@relation_equivalence_pointwise domain).
   pose proof (@relation_equivalence_pointwise env).
   intros * [env_relΓ' [? [env_relΓA]]].
@@ -182,50 +204,65 @@ Proof with intuition.
   inversion_by_head (per_ctx_env env_relΓA); subst.
   rename tail_rel into env_relΓ.
   handle_per_ctx_env_irrel.
-  eexists_rel_subst.
+  eexists_rel_sub.
   intros.
   (on_all_hyp: destruct_rel_by_assumption env_relΓ').
   (on_all_hyp: destruct_rel_by_assumption env_relΓ).
-  econstructor; only 1-2: repeat econstructor; try eexists...
+  econstructor...
 Qed.
 
-Lemma rel_subst_sym : forall {Γ σ σ' Δ},
+#[export]
+Hint Resolve rel_sub_extend : mcltt.
+
+Lemma rel_sub_sym : forall {Γ σ σ' Δ},
     {{ Γ ⊨s σ ≈ σ' : Δ }} ->
     {{ Γ ⊨s σ' ≈ σ : Δ }}.
-Proof with intuition.
+Proof with mautosolve.
   intros * [env_relΓ].
   destruct_conjs.
-  eexists_rel_subst.
+  eexists_rel_sub.
   intros.
   assert (env_relΓ p' p) by (symmetry; eassumption).
   (on_all_hyp: destruct_rel_by_assumption env_relΓ).
-  econstructor; only 1-2: repeat econstructor; try symmetry...
+  econstructor; mauto; symmetry...
 Qed.
 
-Lemma rel_subst_trans : forall {Γ σ σ' σ'' Δ},
+#[export]
+Hint Resolve rel_sub_sym : mcltt.
+
+Lemma rel_sub_trans : forall {Γ σ σ' σ'' Δ},
     {{ Γ ⊨s σ ≈ σ' : Δ }} ->
     {{ Γ ⊨s σ' ≈ σ'' : Δ }} ->
     {{ Γ ⊨s σ ≈ σ'' : Δ }}.
-Proof with intuition.
+Proof with mautosolve.
   pose proof (@relation_equivalence_pointwise domain).
   pose proof (@relation_equivalence_pointwise env).
   intros * [env_relΓ] [].
   destruct_conjs.
   pose (env_relΓ0 := env_relΓ).
   handle_per_ctx_env_irrel.
-  eexists_rel_subst.
+  eexists_rel_sub.
   intros.
   assert (env_relΓ p' p') by (etransitivity; [symmetry |]; eassumption).
   (on_all_hyp: destruct_rel_by_assumption env_relΓ).
   functional_eval_rewrite_clear.
-  econstructor; only 1-2: repeat econstructor; try etransitivity...
+  econstructor; mauto; etransitivity...
 Qed.
 
-Lemma rel_subst_conv : forall {Γ σ σ' Δ Δ'},
+#[export]
+Hint Resolve rel_sub_trans : mcltt.
+
+#[export]
+Instance rel_sub_PER {Γ A} : PER (rel_sub_under_ctx Γ A).
+Proof.
+  split; mauto.
+Qed.
+
+Lemma rel_sub_conv : forall {Γ σ σ' Δ Δ'},
     {{ Γ ⊨s σ ≈ σ' : Δ }} ->
     {{ ⊨ Δ ≈ Δ' }} ->
     {{ Γ ⊨s σ ≈ σ' : Δ' }}.
-Proof with intuition.
+Proof with mautosolve.
   pose proof (@relation_equivalence_pointwise domain).
   pose proof (@relation_equivalence_pointwise env).
   intros * [env_relΓ [? [env_relΔ]]] [].
@@ -233,8 +270,22 @@ Proof with intuition.
   pose (env_relΔ0 := env_relΔ).
   handle_per_ctx_env_irrel.
   assert {{ EF Δ' ≈ Δ' ∈ per_ctx_env ↘ env_relΔ }} by (etransitivity; [symmetry |]; eassumption).
-  eexists_rel_subst.
+  eexists_rel_sub.
   intros.
-  (on_all_hyp: destruct_rel_by_assumption env_relΓ).
-  econstructor; only 1-2: repeat econstructor...
+  (on_all_hyp: destruct_rel_by_assumption env_relΓ)...
+Qed.
+
+#[export]
+Hint Resolve rel_sub_conv : mcltt.
+
+Lemma presup_rel_sub : forall {Γ σ σ' Δ},
+    {{ Γ ⊨s σ ≈ σ' : Δ }} ->
+    {{ ⊨ Γ }} /\ {{ Γ ⊨s σ : Δ }} /\ {{ Γ ⊨s σ' : Δ }} /\ {{ ⊨ Δ }}.
+Proof with mautosolve.
+  intros * [env_relΓ [? [env_relΔ]]].
+  destruct_conjs.
+  repeat split; try solve [eexists; eauto];
+    unfold valid_sub_under_ctx;
+    etransitivity; only 2,3: symmetry;
+    econstructor...
 Qed.
