theories/Core/Completeness/TermStructureCases.v
@@ -7,7 +7,7 @@ Lemma rel_exp_sub_cong : forall {Δ M M' A σ σ' Γ},
     {{ Δ ⊨ M ≈ M' : A }} ->
     {{ Γ ⊨s σ ≈ σ' : Δ }} ->
     {{ Γ ⊨ M[σ] ≈ M'[σ'] : A[σ] }}.
-Proof.
+Proof with mautosolve.
   pose proof (@relation_equivalence_pointwise domain).
   pose proof (@relation_equivalence_pointwise env).
   intros * [env_relΔ] [env_relΓ].
@@ -26,13 +26,16 @@ Proof.
   destruct_by_head rel_typ.
   handle_per_univ_elem_irrel.
   eexists.
-  split; [> econstructor; only 1-2: econstructor; eassumption ..].
+  split...
 Qed.
+
+#[export]
+Hint Resolve rel_exp_sub_cong : mcltt.
 
 Lemma rel_exp_sub_id : forall {Γ M A},
     {{ Γ ⊨ M : A }} ->
     {{ Γ ⊨ M[Id] ≈ M : A }}.
-Proof.
+Proof with mautosolve.
   intros * [env_relΓ].
   destruct_conjs.
   eexists_rel_exp.
@@ -41,16 +44,18 @@ Proof.
   destruct_by_head rel_exp.
   destruct_by_head rel_typ.
   eexists.
-  split; econstructor; try eassumption.
-  repeat econstructor; eassumption.
+  split...
 Qed.
+
+#[export]
+Hint Resolve rel_exp_sub_id : mcltt.
 
 Lemma rel_exp_sub_compose : forall {Γ τ Γ' σ Γ'' M A},
     {{ Γ ⊨s τ : Γ' }} ->
     {{ Γ' ⊨s σ : Γ'' }} ->
     {{ Γ'' ⊨ M : A }} ->
     {{ Γ ⊨ M[σ ∘ τ] ≈ M[σ][τ] : A[σ ∘ τ] }}.
-Proof.
+Proof with mautosolve.
   pose proof (@relation_equivalence_pointwise domain).
   pose proof (@relation_equivalence_pointwise env).
   intros * [env_relΓ [? [env_relΓ']]] [? [? [env_relΓ'']]] [].
@@ -60,8 +65,8 @@ Proof.
   handle_per_ctx_env_irrel.
   eexists_rel_exp.
   intros.
-  assert (env_relΓ p' p) by (eapply per_env_sym; eauto).
-  assert (env_relΓ p p) by (eapply per_env_trans; eauto).
+  assert (env_relΓ p' p) by (symmetry; eassumption).
+  assert (env_relΓ p p) by (etransitivity; eassumption).
   (on_all_hyp: destruct_rel_by_assumption env_relΓ).
   handle_per_univ_elem_irrel.
   (on_all_hyp: destruct_rel_by_assumption env_relΓ').
@@ -72,14 +77,17 @@ Proof.
   destruct_by_head rel_typ.
   handle_per_univ_elem_irrel.
   eexists.
-  split; [> econstructor; only 1-2: repeat econstructor; eassumption ..].
+  split; econstructor...
 Qed.
+
+#[export]
+Hint Resolve rel_exp_sub_compose : mcltt.
 
 Lemma rel_exp_conv : forall {Γ M M' A A' i},
     {{ Γ ⊨ M ≈ M' : A }} ->
     {{ Γ ⊨ A ≈ A' : Type@i }} ->
     {{ Γ ⊨ M ≈ M' : A' }}.
-Proof.
+Proof with mautosolve.
   pose proof (@relation_equivalence_pointwise domain).
   pose proof (@relation_equivalence_pointwise env).
   intros * [env_relΓ] [].
@@ -88,7 +96,7 @@ Proof.
   handle_per_ctx_env_irrel.
   eexists_rel_exp.
   intros.
-  assert (env_relΓ p p) by (eapply per_env_trans; eauto; eapply per_env_sym; eauto).
+  assert (env_relΓ p p) by (etransitivity; [| symmetry]; eassumption).
   (on_all_hyp: destruct_rel_by_assumption env_relΓ).
   destruct_by_head rel_exp.
   destruct_by_head rel_typ.
@@ -96,35 +104,41 @@ Proof.
   destruct_conjs.
   handle_per_univ_elem_irrel.
   eexists.
-  split; econstructor; try eassumption.
-  etransitivity; [symmetry |]; eassumption.
+  split; econstructor; mauto.
+  etransitivity; [symmetry |]...
 Qed.
+
+#[export]
+Hint Resolve rel_exp_conv : mcltt.
 
 Lemma rel_exp_sym : forall {Γ M M' A},
     {{ Γ ⊨ M ≈ M' : A }} ->
     {{ Γ ⊨ M' ≈ M : A }}.
-Proof.
+Proof with mautosolve.
   pose proof (@relation_equivalence_pointwise domain).
   pose proof (@relation_equivalence_pointwise env).
   intros * [env_relΓ].
   destruct_conjs.
   eexists_rel_exp.
   intros.
-  assert (env_relΓ p' p) by (eapply per_env_sym; eauto).
+  assert (env_relΓ p' p) by (symmetry; eauto).
   (on_all_hyp: destruct_rel_by_assumption env_relΓ); destruct_conjs.
   destruct_by_head rel_exp.
   destruct_by_head rel_typ.
   handle_per_univ_elem_irrel.
   eexists.
-  split; econstructor; try eassumption.
-  symmetry; eassumption.
+  split; econstructor; mauto.
+  symmetry...
 Qed.
+
+#[export]
+Hint Resolve rel_exp_sym : mcltt.
 
 Lemma rel_exp_trans : forall {Γ M1 M2 M3 A},
     {{ Γ ⊨ M1 ≈ M2 : A }} ->
     {{ Γ ⊨ M2 ≈ M3 : A }} ->
     {{ Γ ⊨ M1 ≈ M3 : A }}.
-Proof.
+Proof with mautosolve.
   pose proof (@relation_equivalence_pointwise domain).
   pose proof (@relation_equivalence_pointwise env).
   intros * [env_relΓ] [].
@@ -140,16 +154,17 @@ Proof.
   destruct_by_head rel_typ.
   handle_per_univ_elem_irrel.
   eexists.
-  split; econstructor; try eassumption.
-  etransitivity; eassumption.
+  split; econstructor; mauto.
+  etransitivity...
 Qed.
+
+#[export]
+Hint Resolve rel_exp_trans : mcltt.
 
 #[export]
 Instance rel_exp_PER {Γ A} : PER (rel_exp_under_ctx Γ A).
 Proof.
-  split.
-  - auto using rel_exp_sym.
-  - eauto using rel_exp_trans.
+  split; mauto.
 Qed.
 
 Lemma presup_rel_exp : forall {Γ M M' A},
@@ -159,8 +174,8 @@ Proof.
   pose proof (@relation_equivalence_pointwise domain).
   pose proof (@relation_equivalence_pointwise env).
   intros *.
-  assert (Hpart : {{ Γ ⊨ M ≈ M' : A }} -> {{ Γ ⊨ M : A }} /\ {{ Γ ⊨ M' : A }}) by
-    (split; unfold valid_exp_under_ctx; etransitivity; [|symmetry|symmetry|]; eassumption).
+  assert (Hpart : {{ Γ ⊨ M ≈ M' : A }} -> {{ Γ ⊨ M : A }} /\ {{ Γ ⊨ M' : A }})
+    by (split; unfold valid_exp_under_ctx; etransitivity; [|symmetry|symmetry|]; eassumption).
   intros Hrel; repeat split;
     try solve [intuition]; clear Hpart;
     destruct Hrel as [env_relΓ];
@@ -173,9 +188,8 @@ Proof.
     intros.
     (on_all_hyp: destruct_rel_by_assumption env_relΓ).
     eexists (per_univ _).
-    split.
-    + econstructor; only 1-2: repeat econstructor; try eassumption.
-      per_univ_elem_econstructor; eauto.
-      apply Equivalence_Reflexive.
-    + eapply rel_typ_implies_rel_exp; eassumption.
+    split; mauto.
+    econstructor; mauto.
+    per_univ_elem_econstructor; eauto.
+    apply Equivalence_Reflexive.
 Qed.
