theories/Core/Semantic/Realizability.v
@@ -1,7 +1,7 @@
 From Coq Require Import Lia Morphisms_Relations PeanoNat Relation_Definitions.
 From Equations Require Import Equations.
 From Mcltt Require Import Base LibTactics.
-From Mcltt.Core Require Export PER Evaluation Readback.
+From Mcltt.Core Require Export Evaluation NbE PER Readback.
 Import Domain_Notations.
 
 Lemma per_nat_then_per_top : forall {n m},
@@ -36,8 +36,6 @@ Proof with (solve [try (try (eexists; split); econstructor); mauto]).
     destruct_conjs.
     intro s.
     specialize (H2 s) as [? []]...
-  - idtac...
-  - apply_relation_equivalence...
   - destruct IHHunivelem as [? []].
     intro s.
     assert {{ Dom ⇑! A s ≈ ⇑! A' s ∈ in_rel }} by eauto using var_per_bot.
@@ -62,7 +60,6 @@ Proof with (solve [try (try (eexists; split); econstructor); mauto]).
     specialize (H17 (S s)) as [? []]...
   - intro s.
     (on_all_hyp: fun H => destruct (H s) as [? []])...
-  - idtac...
   - intro s.
     inversion_clear_by_head per_ne.
     (on_all_hyp: fun H => specialize (H s) as [? []])...
@@ -98,3 +95,20 @@ Qed.
 
 #[export]
 Hint Resolve per_elem_then_per_top : mcltt.
+
+Lemma per_ctx_then_per_env_initial_env : forall {Γ Γ' env_rel},
+    {{ EF Γ ≈ Γ' ∈ per_ctx_env ↘ env_rel }} ->
+    exists p p', initial_env Γ p /\ initial_env Γ' p' /\ {{ Dom p ≈ p' ∈ env_rel }}.
+Proof.
+  pose proof (@relation_equivalence_pointwise env).
+  induction 1.
+  - do 2 eexists; intuition.
+  - destruct_conjs.
+    (on_all_hyp: destruct_rel_by_assumption tail_rel).
+    do 2 eexists; repeat split; only 1-2: econstructor; eauto.
+    apply_relation_equivalence.
+    eexists.
+    eapply per_bot_then_per_elem; eauto.
+    erewrite per_ctx_respects_length; mauto.
+    eexists; eauto.
+Qed.
